\documentclass{report}

\input{../preamble}
\input{../macros}
\input{../letterfonts}

\usepackage{fancyhdr}
\pagestyle{fancy}

\lhead{\bf Rohan Jain}
\cfoot{}
\rhead{\bf
Putnam Seminar\\
Homework 7}

\begin{document}
\qs{2}{Does the series $$\sum_{n=2}^\infty \frac{1}{n\log^2(n)}$$ converge or diverge?}
\sol We recall Cauchy's condensation test, which yields the following result:

For non-increasing, non-negative $f(x)$, $\sum_{n=1}^{\infty} f(n)$ converges if and only if $\sum_{n=1}^{\infty} 2^nf(2^n)$ converges.

So, we get the following:
\begin{align*}
    \sum_{n=2}^{\infty}\frac{1}{n\log^2(n)} &\leq \sum_{n=2}^{\infty} \frac{2^n}{2^n\log^2(2^n)} = \sum_{n=2}^{\infty} \frac{1}{n^2\log^2(2)}\\
\end{align*}

By the $p$-test, our condensed series converges and therefore so does the original series.


\qs{8}{Evaluate $$\lim_{x \to \infty} (2x)^{1 + 1/2x} - (x)^{1+1/x} - x$$}
\sol We start by factoring out an $x$ and realizing that $x^{1/x} = e^{\ln(x)/x}$. Doing this, we get:
\begin{align*}
    &\lim_{x \to \infty} x (2(2x)^{1/2x} - (x)^{1/x} - 1) \\
    &\lim_{x \to \infty} x(2e^{\ln(2x)/2x} - e^{\ln(x)/x} - 1) \\
    &\lim_{x \to \infty} x \left(2 + \frac{2\ln(2x)}{2x} + O\left(\frac{\ln(x)^2}{x^2}\right) - \left(1 + \frac{\ln(x)}{x} + O\left(\frac{\ln(x)^2}{x^2}\right)\right) - 1\right) \\
    &\lim_{x \to \infty} x \left((2 - 1 - 1) + \left(\frac{\ln(2x)}{x} - \frac{\ln(x)}{x}\right) + \left(O\left(\frac{\ln(x)^2}{x^2}\right) - O\left(\frac{\ln(x)^2}{x^2}\right)\right)\right) \\
    &\lim_{x \to \infty} x\left(\frac{\ln(2)}{x}\right) = \ln(2)
\end{align*}



\end{document}